src/ndep/SymEval.v
@@ -24,6 +24,479 @@ Module Evaluator (B : Heap with Definition mem := W -> B) (ST : SepTheoryX.SepTh
 
     Definition types := bedrock_types ++ types'.
 
+    Record SymEval : Type :=
+    { Predicate : ssignature types pcType stateType
+    ; sym_read  : 
+      forall (hyps args : list (expr types)) (p : expr types), option (expr types)
+    ; sym_write : 
+      forall (hyps args : list (expr types)) (p v : expr types),
+        option (list (expr types))
+    ; sym_read_correct : forall funcs args uvars vars P cs hyps pe ve m s,
+      sym_read hyps args pe = Some ve ->
+      hlist (FalseDefault funcs) hyps ->
+      match applyD (@exprD types funcs uvars vars) (SDomain Predicate) args _ (SDenotation Predicate) with
+        | None => False
+        | Some p => ST.satisfies cs (ST.star p P) s m
+      end ->
+      match exprD funcs uvars vars pe pcType , exprD funcs uvars vars ve pcType with
+        | Some p , Some v =>
+          ReadWord s m p = v 
+        | _ , _ => False
+      end
+    ; sym_write_correct : forall funcs args uvars vars P cs hyps pe ve v m s args',
+      sym_write hyps args pe ve = Some args' ->
+      hlist (FalseDefault funcs) hyps ->
+      exprD funcs uvars vars ve pcType = Some v ->
+      match applyD (@exprD types funcs uvars vars) (SDomain Predicate) args _ (SDenotation Predicate) with
+        | None => False
+        | Some p => ST.satisfies cs (ST.star p P) s m
+      end ->
+      match exprD funcs uvars vars pe pcType with
+        | Some p =>
+          match applyD (@exprD types funcs uvars vars) (SDomain Predicate) args' _ (SDenotation Predicate) with
+            | None => False
+            | Some pr => ST.satisfies cs (ST.star pr P) s (WriteWord s m p v)
+          end
+        | _ => False
+      end
+    }.
+
+    Definition defaultSymEval (P : ssignature types pcType stateType) : SymEval.
+    refine (
+      {| Predicate    := P
+       ; sym_read     := fun _ _ _ => None
+       ; sym_write    := fun _ _ _ _ => None
+       ; sym_read_correct := _
+       ; sym_write_correct := _
+       |}); 
+    abstract (simpl; intros; congruence).
+    Defined.
+
+    Section evaluator.
+      Fixpoint matches (sfuncs : list (ssignature types pcType stateType)) (evals : list SymEval) : Prop :=
+        match evals with
+          | nil => True
+          | e :: es =>
+            match sfuncs with
+              | nil => False
+              | s :: ss => Predicate e = s /\ matches ss es
+            end 
+        end.
+
+      Variable evals : list SymEval.
+
+      Section fold_find.
+        Variable T U : Type.
+        Variable F : nat -> T -> option U.
+        
+        Fixpoint fold_find (m : FM.t T) : option (nat * U) :=
+          match m with 
+            | FM.MLeaf => None
+            | FM.MBranch l k v r =>
+              match F k v with
+                | Some z => Some (k, z)
+                | None => 
+                  match fold_find l with
+                    | None => fold_find r 
+                    | Some k => Some k
+                  end
+              end
+          end.
+      End fold_find.
+
+      Definition symeval_read (hyps : list (expr types)) (p : expr types) (s : SHeap types pcType stateType) 
+        : option (expr types) :=
+        let hyps := hyps ++ pures s in
+        let res := 
+          fold_find (fun k v => 
+            match nth_error evals k with
+              | Some ev =>
+                let reader := sym_read ev hyps in
+                  List.fold_left (fun acc args =>
+                    match acc with
+                      | Some _ => acc
+                      | None => reader args p 
+                    end) v None
+              | _ => None
+            end)
+          (impures s)
+        in match res with
+             | None => None
+             | Some a => Some (snd a)
+           end.
+
+      Variable funcs : functions types.
+      Variable sfuncs : list (ssignature types pcType stateType).
+      Hypothesis evals_matches : matches sfuncs evals.
+
+      Theorem symeval_read_correct : forall hyps pe s ve,
+        symeval_read hyps pe s = Some ve ->
+        hlist (FalseDefault funcs) hyps ->
+        forall uvars vars cs stn m,
+        ST.satisfies cs (@sexprD types funcs pcType stateType sfuncs (SEP.sheapD s) uvars vars) stn m -> 
+        match exprD funcs uvars vars ve pcType , exprD funcs uvars vars pe pcType with
+          | Some v , Some p => ReadWord stn m p = v 
+          | _ , _ => False
+        end.
+      Proof.
+(*
+        Opaque tvarD.
+        unfold symeval_read. destruct s; simpl.
+        induction impures0; simpl in *.
+          intros; congruence.
+
+          intros. 
+          Lemma satisfies_lemma : forall cs stn funcs sfuncs uvars vars0 m mp k v other0 pures0,
+            ST.satisfies cs
+            (sexprD funcs sfuncs
+              (sheapD
+                {| impures := mp ;
+                   pures := pures0;
+                   other := other0 |}) uvars vars0) stn m ->
+            FM.find k mp = Some v ->
+            ST.satisfies cs 
+            (sexprD funcs sfuncs (starred (Func k) v (@Emp types pcType stateType)) uvars vars0) stn m.
+          Proof.
+            clear. induction mp; simpl; intros.
+              congruence.
+
+              eapply ST.satisfies_himp in H.
+              2: eapply ST.heq_himp; eapply sheapD_sheapD'.
+              unfold sheapD' in H. simpl in H.
+          generalize H0. unfold sheapD in H0. simpl in H0.
+
+              destruct (Compare_dec.lt_eq_lt_dec k n). destruct s.
+              eapply IHmp1 in H0; eauto.
+              Focus 2.
+
+eapply ST.satisfies_himp in H0.
+          2: eapply ST.heq_himp; eapply sheapD_sheapD'.
+          unfold sheapD' in H0. simpl in H0.
+          generalize H0. unfold sheapD in H0. simpl in H0.
+          
+
+          assert (ST.satisfies cs (sexprD funcs sfuncs (sheapD {| impures := impures0_1 ; pures := pures0 ; other := other0 |}) uvars vars0) stn m).
+          cut (ST.satisfies (sexprD funcs sfuncs (sheapD {| impures := impures0_2 ; pures := pures0 ; other := other0 |}) uvars vars0) cs stn m).
+          Focus.
+
+          Ltac head x :=
+            match x with
+              | match ?y with
+                  | Some _ => _
+                  | None => _
+                end => head y
+              | _ => x
+            end.
+
+          Print ST.
+          Ltac more :=
+          repeat match goal with
+                   | [  H' : _ |- _ ] => 
+                     specialize (H' _ (refl_equal _))
+                   | [ H : hlist (FalseDefault _) _, H' : _  |- _ ] =>
+                     specialize (H' H)
+                   | [ H : ST.satisfies _ _ _ _ , H' : _  |- _ ] =>
+                     specialize (H' _ _ _ _ _ H)
+                   | _ => solve [ eauto ] 
+                   | [ H : Some _ = Some _ |- _ ] => inversion H; clear H; try subst
+                   | [ H : forall x, None = Some x -> _ |- _ ] => clear H
+                   | [ H : context [ match ?X with
+                                       | Some _ => _
+                                       | None => _
+                                     end ] |- _ ] =>
+                   let X := head X in
+                     match X with 
+                       | fold_left _ _ _ =>
+                         generalize dependent H; case_eq (X); intros
+                       | fold_find _ _ =>
+                         generalize dependent X; let H := fresh in intro H; destruct H; intros
+(*
+                          (idtac "matched fold_find";
+                          intros; generalize dependent H; case_eq X;
+                            [ idtac "a"; let z := fresh "p" in intro z; let H' := fresh in intro H'; idtac "trying to rw"; 
+                              let v := eval unfold H' in H' in idtac v ; rewrite H' in *; idtac "a done" |
+                              idtac "b"; let H' := fresh in intros H'; rewrite H' in * ; idtac "b done" ]; intros ; idtac "completed")
+*)
+
+                       | exprD _ _ _ _ _ => fail 2
+                     end
+                   | _ => congruence
+                 end; eauto.
+          destruct (nth_error evals n); intros; more; try destruct o; more.
+          Print sheapD.
+          Lemma scan_function_correct : forall uvars vars0 t cs stn m pe ve k hyps s acc,
+            fold_left
+            (fun (acc : option (expr types)) (args : list (expr types)) =>
+              match acc with
+                | Some _ => acc
+                | None => sym_read s hyps args pe
+              end) t acc = Some ve ->
+            match acc with
+              | None => True
+              | Some ve =>
+                match exprD funcs uvars vars0 ve pcType with
+                  | Some v =>
+                    match exprD funcs uvars vars0 pe pcType with
+                      | Some p0 => ReadWord stn m p0 = v
+                      | None => False
+                    end
+                  | None => False
+                end
+            end ->                
+            nth_error evals k = Some (Some s) ->
+            ST.satisfies (@sexprD types funcs pcType stateType sfuncs (starred' (Func k) t Emp) uvars vars0) cs stn m ->
+            match exprD funcs uvars vars0 ve pcType with
+              | Some v =>
+                match exprD funcs uvars vars0 pe pcType with
+                  | Some p0 => ReadWord stn m p0 = v
+                  | None => False
+                end
+              | None => False
+            end.
+          Proof.
+            induction t; simpl in *.
+              intros; subst; auto.
+
+              intros. destruct acc.
+              assert (e = ve).
+              generalize H. clear.
+              induction t; eauto; simpl; congruence.
+              subst. eauto.
+              eapply IHt; eauto.
+              assert (nth_error sfuncs k = Some (Predicate s)).
+              Focus.
+              generalize H1. generalize evals_matches. clear. generalize sfuncs. clear. induction evals; simpl.
+                destruct k; intros; simpl in *. inversion H1. inversion H1.
+                destruct sfuncs; simpl in *; intros; try intuition.
+                destruct k; simpl in *. inversion H1; clear H1; subst. subst. reflexivity.
+                eapply IHl in H0; eauto.
+                
+
+                destruct k. simpl. inversion 2. subst. destruct sfuncs; auto.
+                simpl in *; eauto. intuition. subst. reflexivity.
+                destruct sfuncs; intuition. 
+
+              simpl in *. dest
+*)
+      Admitted.
+
+      Fixpoint map_maybe_map (T : Type) (F : nat -> T -> option T) (m : FM.t T) 
+        : option (FM.t T) :=
+        match m with
+          | FM.MLeaf => None
+          | FM.MBranch l k v r =>
+            match F k v with
+              | Some v' => Some (FM.MBranch _ l k v' r)
+              | None => 
+                match map_maybe_map F l with
+                  | Some l' => Some (FM.MBranch _ l' k v r)
+                  | None => 
+                    match map_maybe_map F r with
+                      | Some r' => Some (FM.MBranch _ l k v r')
+                      | None => None
+                    end
+                end
+            end
+        end.
+        
+      Fixpoint list_maybe_map (T : Type) (F : T -> option T) (m : list T) 
+        : option (list T) :=
+        match m with
+          | nil => None
+          | a :: b => 
+            match F a with
+              | None => match list_maybe_map F b with
+                          | None => None
+                          | Some b' => Some (a :: b')
+                        end
+              | Some a' => Some (a' :: b)
+            end
+        end.
+
+      Definition symeval_write (hyps : list (expr types)) (p v : expr types) 
+        (s : SHeap types pcType stateType) : option (SHeap types pcType stateType) :=
+        let hyps := hyps ++ pures s in
+        let res := 
+          map_maybe_map (fun k =>
+            match nth_error evals k with 
+              | None => fun _ => None
+              | Some ev =>
+                let writer := sym_write ev hyps in
+                list_maybe_map (fun args =>
+                  writer args p v)
+            end) (impures s)
+        in
+        match res with
+          | None => None
+          | Some i => Some {| impures := i ; pures := pures s ; other := other s |}
+        end.
+
+      Theorem symeval_write_correct : forall hyps pe s s' ve,
+        symeval_write hyps pe ve s = Some s' ->
+        hlist (FalseDefault funcs) hyps ->
+        forall uvars vars cs stn m,
+        ST.satisfies cs (@sexprD types funcs pcType stateType sfuncs (SEP.sheapD s) uvars vars) stn m -> 
+        match exprD funcs uvars vars ve pcType , exprD funcs uvars vars pe pcType with
+          | Some v , Some p => 
+            ST.satisfies cs (@sexprD types funcs pcType stateType sfuncs (SEP.sheapD s) uvars vars) stn (WriteWord stn m p v)
+          | _ , _ => False
+        end.
+      Proof.
+      Admitted.
+  (*
+End Evaluator.
+*)
+    End evaluator.
+  End typed.
+
+  Section ptsto32_sym_eval.
+    Variable types' : list type.
+    
+    Definition ptsto32_Predicate : ssignature (types types') pcType stateType :=
+      Build_ssignature (types types') pcType stateType (pcType :: pcType :: nil) (@ptsto32 nil).
+    
+    (** Let's see how this works with ptsto **)
+    Definition ptsto32_sym_read (hyps args : list (expr (types types'))) (p : expr (types types')) : option (expr (types types')) :=
+      match args with
+        | p' :: v :: nil =>
+          if seq_dec p p' then Some v else None
+        | _ => None
+      end.
+    
+    Definition ptsto32_sym_write (hyps : list (expr (types types'))) (args : list (expr (types types'))) (p v : expr (types types')) : option (list (expr (types types'))) :=
+      match args with
+        | p' :: _ :: nil =>
+          if seq_dec p p' then Some (p' :: v :: nil) else None
+        | _ => None
+      end.
+
+    Require Import PropXTac.
+
+    Theorem ptsto32_sym_read_correct : forall (funcs : functions (types types'))
+      (args : list (expr (types types'))) (uvars vars0 : env (types types'))
+      (P : hprop (tvarD (types types') pcType)
+        (tvarD (types types') stateType) nil)
+      (cs : PropX.codeSpec (tvarD (types types') pcType)
+        (tvarD (types types') stateType))
+      (hyps : list (expr (types types'))) (pe ve : expr (types types'))
+      (m : BedrockHeap.mem) (s : settings),
+      ptsto32_sym_read hyps args pe = Some ve ->
+      hlist (FalseDefault funcs) hyps ->
+      match
+        applyD (exprD funcs uvars vars0) (SDomain ptsto32_Predicate) args
+        (hprop (tvarD (types types') pcType) (tvarD (types types') stateType)
+          nil) (SDenotation ptsto32_Predicate)
+        with
+        | Some p => ST.satisfies cs (star p P) s m
+        | None => False
+      end ->
+      match exprD funcs uvars vars0 pe pcType with
+        | Some p =>
+          match exprD funcs uvars vars0 ve pcType with
+            | Some v => ReadWord s m p = v
+            | None => False
+          end
+        | None => False
+      end.
+    Proof.
+      unfold ptsto32_Predicate; simpl in *; intros.
+      destruct args; simpl in *; try congruence.
+      destruct args; simpl in *; try congruence.
+      destruct args; simpl in *; try congruence.
+      destruct (expr_seq_dec pe e); try congruence.
+      inversion H; clear H; subst.
+      destruct (exprD funcs uvars vars0 e pcType); auto.
+      destruct (exprD funcs uvars vars0 ve pcType); auto.
+      eapply ST.satisfies_star in H0. destruct H0. clear H0.
+      destruct H as [ ? [ ? ? ] ]. (** Breaks abstraction **)
+      propxFo. unfold implode in H6. subst.
+      repeat match goal with 
+               | [ H : smem_get _ _ = _ |- _ ] =>
+                 eapply satisfies_get in H; [ | eassumption ]; unfold BedrockHeap.mem_get in H; inversion H; subst
+             end;
+      eapply ReadWordFootprint; simpl; auto.
+    Qed.
+
+    Theorem ptsto32_sym_write_correct : forall (funcs : functions (types types'))
+      (args : list (expr (types types'))) (uvars vars0 : env (types types'))
+      (P : hprop (tvarD (types types') pcType)
+        (tvarD (types types') stateType) nil)
+      (cs : PropX.codeSpec (tvarD (types types') pcType)
+        (tvarD (types types') stateType))
+      (hyps : list (expr (types types'))) (pe ve : expr (types types'))
+      (v : tvarD (types types') pcType) (m : BedrockHeap.mem) 
+      (s : settings) (args' : list (expr (types types'))),
+      ptsto32_sym_write hyps args pe ve = Some args' ->
+      hlist (FalseDefault funcs) hyps ->
+      exprD funcs uvars vars0 ve pcType = Some v ->
+      match
+        applyD (exprD funcs uvars vars0) (SDomain ptsto32_Predicate) args
+        (hprop (tvarD (types types') pcType) (tvarD (types types') stateType)
+          nil) (SDenotation ptsto32_Predicate)
+        with
+        | Some p => ST.satisfies cs (star p P) s m
+        | None => False
+      end ->
+      match exprD funcs uvars vars0 pe pcType with
+        | Some p =>
+          match
+            applyD (exprD funcs uvars vars0) (SDomain ptsto32_Predicate) args'
+            (hprop (tvarD (types types') pcType)
+              (tvarD (types types') stateType) nil)
+            (SDenotation ptsto32_Predicate)
+            with
+            | Some pr => ST.satisfies cs (star pr P) s (WriteWord s m p v)
+            | None => False
+          end
+        | None => False
+      end.
+    Proof.
+      unfold ptsto32_Predicate; simpl in *; intros.
+      destruct args; simpl in *; try congruence.
+      destruct args; simpl in *; try congruence.
+      destruct args; simpl in *; try congruence.
+      destruct (expr_seq_dec pe e); try congruence.
+      inversion H; clear H; subst. simpl.
+      destruct (exprD funcs uvars vars0 e pcType); auto.
+      destruct (exprD funcs uvars vars0 e0 pcType); try tauto.
+      rewrite H0. clear H0.
+    Admitted.
+      
+    Definition SymEval_ptsto32 : SymEval types' :=
+      {| Predicate := ptsto32_Predicate 
+       ; sym_read  := ptsto32_sym_read
+       ; sym_write := ptsto32_sym_write
+       ; sym_read_correct := ptsto32_sym_read_correct
+       ; sym_write_correct := ptsto32_sym_write_correct
+       |}.
+  End ptsto32_sym_eval.
+
+  Section Tests.
+
+    Require Import PropX.
+    Goal forall specs stn p v x,
+      PropX.interp specs (![ptsto32 _ p v]%PropX (stn, x)) ->
+      ReadWord stn (Mem x) p = v.
+    Proof.
+      intros.
+      match goal with
+        | [ |- context [ ReadWord ?STN ?M ?P ] ] =>
+          match goal with
+            | [ H : interp ?CS (![?S] (STN, ?ST)) |- _ ] =>
+              let m := eval simpl in (Mem ST) in 
+              match M with
+                | m => idtac "found!"
+              end
+          end
+      end.
+      generalize (symeval_read_correct).
+    Abort.
+      
+    End Tests.
+
+
+(* This is the instantiation of the old evaluator.
+  Section ptsto32_sym_eval.
     Definition denotesTo (sfuncs : list (ssignature types pcType stateType)) (f : nat) 
       (Predicate : ssignature types pcType stateType) : Prop :=
       nth_error sfuncs f = Some Predicate.
@@ -68,14 +541,8 @@ Module Evaluator (B : Heap with Definition mem := W -> B) (ST : SepTheoryX.SepTh
           | _ => False
         end
       }.
-  End typed.
-(*
-End Evaluator.
-*)
 
 
-
-  Section ptsto32_sym_eval.
     Definition btypes : list type := bedrock_types.
     Variable types : list type.
 
@@ -191,3 +658,5 @@ End Evaluator.
       |}.
 
   End  ptsto32_sym_eval.
+
+*)
